Core/Metatheory/SpineType.lean
@@ -11,6 +11,33 @@ import Core.Metatheory.GlobalWf
 import Core.Metatheory.Uniqueness
 import Core.Metatheory.Inversion
 
+theorem spine_has_base_type {t : Term} :
+  G&Δ,Γ ⊢ t.apply sp : T ->
+  ∃ B, G&Δ,Γ ⊢ t : B ∧ TypeMatch B T
+:= by
+  intro j; induction sp generalizing t T <;> simp [Term.apply] at *
+  case nil =>
+    exists T; apply And.intro j
+    apply TypeMatch.refl
+  case cons hd tl ih =>
+    cases hd
+    case type A =>
+      obtain ⟨B, ih1, ih2⟩ := ih j
+      cases ih1; case _ K C q1 q2 q3 =>
+      subst q3; exists ∀[K]C
+      apply And.intro q2
+      apply TypeMatch.all A ih2
+    case term a =>
+      obtain ⟨B, ih1, ih2⟩ := ih j
+      cases ih1; case _ A q1 q2 q3 =>
+      exists A -:> B; apply And.intro q3
+      apply TypeMatch.arrow ih2
+    case oterm a =>
+      obtain ⟨B, ih1, ih2⟩ := ih j
+      cases ih1; case _ A q1 q2 q3 =>
+      exists A -:> B; apply And.intro q3
+      apply TypeMatch.arrow ih2
+
 theorem SpineType.apply :
   G&Δ, Γ ⊢ t : T ->
   SpineType G Δ Γ sp B T ->
